Added RelVal and RV and disable enum, tuple, record and union

theories/Syntax/TypeDecl.v
@@ -54,9 +54,9 @@ Module ty.
 
   Class TypeDeclKit : Type :=
     { (* Type constructor names. *)
-      enumi    : Set;           (* Names of enum type constructors. *)
-      unioni   : Set;           (* Names of union type constructors. *)
-      recordi  : Set;           (* Names of record type constructors. *)
+      (* enumi    : Set;           (* Names of enum type constructors. *) *)
+      (* unioni   : Set;           (* Names of union type constructors. *) *)
+      (* recordi  : Set;           (* Names of record type constructors. *) *)
     }.
 
   Section WithTypeDecl.
@@ -74,11 +74,11 @@ Module ty.
     | prod (σ τ : Ty)
     | sum  (σ τ : Ty)
     | unit
-    | enum (E : enumi)
+    (* | enum (E : enumi) *)
     | bvec (n : nat)
-    | tuple (σs : Ctx Ty)
-    | union (U : unioni)
-    | record (R : recordi)
+    (* | tuple (σs : Ctx Ty) *)
+    (* | union (U : unioni) *)
+    (* | record (R : recordi) *)
     .
     Derive NoConfusion for Ty.
 
@@ -95,11 +95,11 @@ Module ty.
       Hypothesis (P_prod   : forall σ τ, P σ -> P τ -> P (prod σ τ)).
       Hypothesis (P_sum    : forall σ τ, P σ -> P τ -> P (sum σ τ)).
       Hypothesis (P_unit   : P unit).
-      Hypothesis (P_enum   : forall E, P (enum E)).
+      (* Hypothesis (P_enum   : forall E, P (enum E)). *)
       Hypothesis (P_bvec   : forall n, P (bvec n)).
-      Hypothesis (P_tuple  : forall σs (IH : ctx.All P σs), P (tuple σs)).
-      Hypothesis (P_union  : forall U, P (union U)).
-      Hypothesis (P_record : forall R, P (record R)).
+      (* Hypothesis (P_tuple  : forall σs (IH : ctx.All P σs), P (tuple σs)). *)
+      (* Hypothesis (P_union  : forall U, P (union U)). *)
+      (* Hypothesis (P_record : forall R, P (record R)). *)
 
       Fixpoint Ty_rect (σ : Ty) : P σ :=
         match σ with
@@ -110,11 +110,11 @@ Module ty.
         | prod σ τ => ltac:(apply P_prod; auto)
         | sum σ τ  => ltac:(apply P_sum; auto)
         | unit     => ltac:(apply P_unit; auto)
-        | enum E   => ltac:(apply P_enum; auto)
+        (* | enum E   => ltac:(apply P_enum; auto) *)
         | bvec n   => ltac:(apply P_bvec; auto)
-        | tuple σs => ltac:(apply P_tuple, ctx.all_intro, Ty_rect)
-        | union U  => ltac:(apply P_union; auto)
-        | record R => ltac:(apply P_record; auto)
+        (* | tuple σs => ltac:(apply P_tuple, ctx.all_intro, Ty_rect) *)
+        (* | union U  => ltac:(apply P_union; auto) *)
+        (* | record R => ltac:(apply P_record; auto) *)
         end.
 
     End Ty_rect.
@@ -126,11 +126,11 @@ Module ty.
 
   Class TypeDenoteKit (TDC : TypeDeclKit) : Type :=
     { (* Mapping enum type constructor names to enum types *)
-      enumt   : enumi -> Set;
-      (* Mapping union type constructor names to union types *)
-      uniont  : unioni -> Set;
-      (* Mapping record type constructor names to record types *)
-      recordt : recordi -> Set;
+      (* enumt   : enumi -> Set; *)
+      (* (* Mapping union type constructor names to union types *) *)
+      (* uniont  : unioni -> Set; *)
+      (* (* Mapping record type constructor names to record types *) *)
+      (* recordt : recordi -> Set; *)
     }.
 
   Section WithTypeDenote.
@@ -147,64 +147,172 @@ Module ty.
       | prod σ1 σ2 => Val σ1 * Val σ2
       | sum σ1 σ2 => Val σ1 + Val σ2
       | unit => Datatypes.unit
-      | enum E => enumt E
+      (* | enum E => enumt E *)
       | bvec n => bv n
-      | tuple σs => EnvRec Val σs
-      | union U => uniont U
-      | record R => recordt R
+      (* | tuple σs => EnvRec Val σs *)
+      (* | union U => uniont U *)
+      (* | record R => recordt R *)
       end%type.
+
+    #[universes(template)]
+      (* Set Universe Polymorphism. *)
+      Inductive RV (A : Type) : Type :=
+    | SyncVal : A -> RV A
+    | NonSyncVal : A -> A -> RV A
+    .
+    Global Arguments SyncVal {A}.
+    Global Arguments NonSyncVal {A}.
+
+    Definition projLeftRV {A} (rv : RV A) : A :=
+      match rv with
+      | SyncVal v => v
+      | NonSyncVal vl _ => vl
+      end.
+
+    Definition projRightRV {A} (rv : RV A) : A :=
+      match rv with
+      | SyncVal v => v
+      | NonSyncVal _ vr => vr
+      end.
+
+    Definition RelVal {TDC : TypeDeclKit} {TDN : TypeDenoteKit TDC} (τ : Ty) : Set :=
+      RV (Val τ)
+    .
+
+    Definition projLeft {A} (rv : RelVal A) : Val A :=
+      projLeftRV rv.
+
+    Definition projRight {A} (rv : RelVal A) : Val A :=
+      projRightRV rv.
+
+    Definition liftUnOpRV {A B} (f : A -> B) (rv : RV A) : RV B :=
+      match rv with
+      | (SyncVal v) => SyncVal (f v)
+      | (NonSyncVal vl vr) => NonSyncVal (f vl) (f vr)
+      end.
+
+    Definition liftBinOpRV {A B C} (f : A -> B -> C) (rv1 : RV A) (rv2 : RV B) : RV C :=
+      match (rv1 , rv2) with
+      | (SyncVal v1 , SyncVal v2) => SyncVal (f v1 v2)
+      | (_ , _) => NonSyncVal (f (projLeftRV rv1) (projLeftRV rv2)) (f (projRightRV rv1) (projRightRV rv2))
+      end.
+
+    Definition liftUnOp {A B} (f : Val A -> Val B) (rv : RelVal A) : RelVal B :=
+      liftUnOpRV f rv.
+
+    Definition liftBinOp {A B C} (f : Val A -> Val B -> Val C) (rv1 : RelVal A) (rv2 : RelVal B) : RelVal C :=
+      liftBinOpRV f rv1 rv2.
+
+    Definition valToRelVal {σ} : Val σ -> RelVal σ :=
+      SyncVal.
+
+    Fixpoint listOfRVToRVOfList {A} (rv_list : (Datatypes.list (RV A))) : RV (Datatypes.list A) :=
+      match rv_list with
+      | nil => SyncVal nil
+      | (x :: l)%list => liftBinOpRV cons x (listOfRVToRVOfList l)
+      end.
+
+    Definition listOfRelValToRelValOfList {A} (rv_list : (Datatypes.list (RelVal A))) : RelVal (list A) :=
+      listOfRVToRVOfList rv_list.
+
+    Definition RVOfPairToPairOfRV {σ1 σ2} (rv : RV (σ1 * σ2)) : RV σ1 * RV σ2 :=
+      match rv with
+      | SyncVal (a , b) => (SyncVal a, SyncVal b)
+      | NonSyncVal (a1, b1) (a2, b2) => (NonSyncVal a1 a2, NonSyncVal b1 b2)
+      end.
+
+    Definition pairOfRVToRVOfPair {σ1 σ2} (rv_pair : RV σ1 * RV σ2) : RV (σ1 * σ2) :=
+      match rv_pair with
+      | (SyncVal v1 , SyncVal v2) => SyncVal (v1, v2)
+      | (rv1, rv2) => NonSyncVal (projLeftRV rv1, projLeftRV rv2) (projRightRV rv1, projRightRV rv2)
+      end.
+
+    Definition RelValOfPairToPairOfRelVal {σ1 σ2} (rv : RelVal (prod σ1 σ2)) : RelVal σ1 * RelVal σ2 :=
+      RVOfPairToPairOfRV rv.
+
+    Definition pairOfRelValToRelValOfPair {σ1 σ2} (rv_pair : RelVal σ1 * RelVal σ2) : RelVal (prod σ1 σ2) :=
+      pairOfRVToRVOfPair rv_pair.
+
+    Definition isSyncValRV {σ} (rv : RV σ) : Datatypes.bool :=
+      match rv with
+      | SyncVal _ => true
+      | NonSyncVal _ _ => false
+      end.
+
+    Definition isSyncVal {σ} : RelVal σ -> Datatypes.bool :=
+      isSyncValRV.
+
+    Definition isSyncValPropRV {σ} (v : RV σ) : Prop :=
+      match v with
+      | SyncVal _ => True
+      | NonSyncVal _ _ => False
+      end.
+
+    Definition isSyncValProp {σ} : RelVal σ -> Prop :=
+      isSyncValPropRV.
+    
+
+    Fixpoint vecOfRVToRVOfVec {n} (rv_vec : Vector.t (RV (Val bool)) n) : RV (Val (ty.bvec n)) :=
+      match rv_vec with
+      | Vector.nil => SyncVal bv.nil
+      | Vector.cons x l => liftBinOpRV (A := Val bool) (B := Val (bvec _)) (C := Val (bvec _)) (bv.cons (n := _)) x (vecOfRVToRVOfVec l)
+      end.
+
+    Fixpoint vecOfRelValToRelValOfVec {n} (rv_vec : Vector.t (RelVal bool) n) : RelVal (ty.bvec n) :=
+      vecOfRVToRVOfVec rv_vec
+      .
 
   End WithTypeDenote.
 
   Class TypeDefKit {TDC : TypeDeclKit} (TDN : TypeDenoteKit TDC) : Type :=
-    { enum_eqdec   : EqDec enumi;
-      union_eqdec  : EqDec unioni;
-      record_eqdec : EqDec recordi;
+    { (* enum_eqdec   : EqDec enumi; *)
+      (* union_eqdec  : EqDec unioni; *)
+      (* record_eqdec : EqDec recordi; *)
 
-      enumt_eqdec E  : EqDec (enumt E);
-      enumt_finite E : finite.Finite (enumt E);
+      (* enumt_eqdec E  : EqDec (enumt E); *)
+      (* enumt_finite E : finite.Finite (enumt E); *)
 
-      uniont_eqdec U  : EqDec (uniont U);
-      (* Names of union data constructors. *)
-      unionk          : unioni -> Set;
-      unionk_eqdec U  : EqDec (unionk U);
-      unionk_finite U : finite.Finite (unionk U);
-      unionk_ty U     : unionk U -> Ty;
+      (* uniont_eqdec U  : EqDec (uniont U); *)
+      (* (* Names of union data constructors. *) *)
+      (* unionk          : unioni -> Set; *)
+      (* unionk_eqdec U  : EqDec (unionk U); *)
+      (* unionk_finite U : finite.Finite (unionk U); *)
+      (* unionk_ty U     : unionk U -> Ty; *)
 
-      recordt_eqdec R  : EqDec (recordt R);
-      (* Record field names. *)
-      recordf          : Set;
-      (* Record field types. *)
-      recordf_ty       : recordi -> NCtx recordf Ty;
+      (* recordt_eqdec R  : EqDec (recordt R); *)
+      (* (* Record field names. *) *)
+      (* recordf          : Set; *)
+      (* (* Record field types. *) *)
+      (* recordf_ty       : recordi -> NCtx recordf Ty; *)
 
-      (* Union types. *)
-      (* Union data constructor field type *)
-      unionv_fold U   : { K : unionk U & Val (unionk_ty U K) } -> uniont U;
-      unionv_unfold U : uniont U -> { K : unionk U & Val (unionk_ty U K) };
+      (* (* Union types. *) *)
+      (* (* Union data constructor field type *) *)
+      (* unionv_fold U   : { K : unionk U & Val (unionk_ty U K) } -> uniont U; *)
+      (* unionv_unfold U : uniont U -> { K : unionk U & Val (unionk_ty U K) }; *)
 
-      (* Record types. *)
-      recordv_fold R   : NamedEnv Val (recordf_ty R) -> recordt R;
-      recordv_unfold R : recordt R -> NamedEnv Val (recordf_ty R);
+      (* (* Record types. *) *)
+      (* recordv_fold R   : NamedEnv Val (recordf_ty R) -> recordt R; *)
+      (* recordv_unfold R : recordt R -> NamedEnv Val (recordf_ty R); *)
 
-      unionv_fold_unfold U K : unionv_fold U (unionv_unfold U K) = K;
-      unionv_unfold_fold U K : unionv_unfold U (unionv_fold U K) = K;
+      (* unionv_fold_unfold U K : unionv_fold U (unionv_unfold U K) = K; *)
+      (* unionv_unfold_fold U K : unionv_unfold U (unionv_fold U K) = K; *)
 
-      recordv_fold_unfold R v : recordv_fold R (recordv_unfold R v) = v;
-      recordv_unfold_fold R v : recordv_unfold R (recordv_fold R v) = v;
+      (* recordv_fold_unfold R v : recordv_fold R (recordv_unfold R v) = v; *)
+      (* recordv_unfold_fold R v : recordv_unfold R (recordv_fold R v) = v; *)
     }.
 
   (* Coq 8.16 will start generating coercions for [:>] in Class definitions. Not
      sure what the implications are and if we want that. For now, manually
      declare the necessary fields as superclass instances. *)
-  #[export] Existing Instance enum_eqdec.
-  #[export] Existing Instance union_eqdec.
-  #[export] Existing Instance record_eqdec.
-  #[export] Existing Instance enumt_eqdec.
-  #[export] Existing Instance enumt_finite.
-  #[export] Existing Instance uniont_eqdec.
-  #[export] Existing Instance unionk_eqdec.
-  #[export] Existing Instance unionk_finite.
-  #[export] Existing Instance recordt_eqdec.
+  (* #[export] Existing Instance enum_eqdec. *)
+  (* #[export] Existing Instance union_eqdec. *)
+  (* #[export] Existing Instance record_eqdec. *)
+  (* #[export] Existing Instance enumt_eqdec. *)
+  (* #[export] Existing Instance enumt_finite. *)
+  (* #[export] Existing Instance uniont_eqdec. *)
+  (* #[export] Existing Instance unionk_eqdec. *)
+  (* #[export] Existing Instance unionk_finite. *)
+  (* #[export] Existing Instance recordt_eqdec. *)
 
   Section WithTypeDef.
 
@@ -222,13 +330,13 @@ Module ty.
         | prod σ1 σ2 , prod τ1 τ2 => f_equal2_dec prod noConfusion_inv (ty_eqdec σ1 τ1) (ty_eqdec σ2 τ2)
         | sum σ1 σ2  , sum τ1 τ2  => f_equal2_dec sum noConfusion_inv (ty_eqdec σ1 τ1) (ty_eqdec σ2 τ2)
         | unit       , unit       => left eq_refl
-        | enum E1    , enum E2    => f_equal_dec enum noConfusion_inv (eq_dec E1 E2)
+        (* | enum E1    , enum E2    => f_equal_dec enum noConfusion_inv (eq_dec E1 E2) *)
         | bvec n1    , bvec n2    => f_equal_dec bvec noConfusion_inv (eq_dec n1 n2)
-        | tuple σs   , tuple τs   => f_equal_dec
-                                       tuple noConfusion_inv
-                                       (eq_dec (EqDec := ctx.eq_dec_ctx ty_eqdec) σs τs)
-        | union U1   , union U2   => f_equal_dec union noConfusion_inv (eq_dec U1 U2)
-        | record R1  , record R2  => f_equal_dec record noConfusion_inv (eq_dec R1 R2)
+        (* | tuple σs   , tuple τs   => f_equal_dec *)
+        (*                                tuple noConfusion_inv *)
+        (*                                (eq_dec (EqDec := ctx.eq_dec_ctx ty_eqdec) σs τs) *)
+        (* | union U1   , union U2   => f_equal_dec union noConfusion_inv (eq_dec U1 U2) *)
+        (* | record R1  , record R2  => f_equal_dec record noConfusion_inv (eq_dec R1 R2) *)
         | _          , _          => right noConfusion_inv
         end.
 
@@ -242,51 +350,99 @@ Module ty.
         | prod σ τ => eq_dec (A := Datatypes.prod (Val σ) (Val τ))
         | sum σ τ  => eq_dec (A := Datatypes.sum (Val σ) (Val τ))
         | unit     => eq_dec (A := Datatypes.unit)
-        | enum E   => eq_dec (A := enumt E)
+        (* | enum E   => eq_dec (A := enumt E) *)
         | bvec n   => eq_dec (A := bv n)
-        | tuple σs => ctx.Ctx_rect
-                        (fun τs => EqDec (EnvRec Val τs))
-                        (eq_dec (A := Datatypes.unit))
-                        (fun τs IHτs τ =>
-                           @eq_dec
-                             (Datatypes.prod (EnvRec Val τs) (Val τ))
-                             (prod_eqdec IHτs (eqd τ)))
-                        σs
-        | union U  => eq_dec (A := uniont U)
-        | record R => eq_dec (A := recordt R)
+        (* | tuple σs => ctx.Ctx_rect *)
+        (*                 (fun τs => EqDec (EnvRec Val τs)) *)
+        (*                 (eq_dec (A := Datatypes.unit)) *)
+        (*                 (fun τs IHτs τ => *)
+        (*                    @eq_dec *)
+        (*                      (Datatypes.prod (EnvRec Val τs) (Val τ)) *)
+        (*                      (prod_eqdec IHτs (eqd τ))) *)
+        (*                 σs *)
+        (* | union U  => eq_dec (A := uniont U) *)
+        (* | record R => eq_dec (A := recordt R) *)
         end.
 
-    Lemma unionv_fold_inj {U} (v1 v2 : {K : unionk U & Val (unionk_ty U K)}) :
-      unionv_fold U v1 = unionv_fold U v2 <-> v1 = v2.
-    Proof.
-      split; intro H; [|now f_equal].
-      apply (f_equal (unionv_unfold U)) in H.
-      now rewrite !unionv_unfold_fold in H.
-    Qed.
+    #[export] Instance RV_eq_dec : forall σ, EqDec (Val σ) :=
+      fix eqd σ :=
+        match σ with
+        | int      => eq_dec (A := Z)
+        | bool     => eq_dec (A := Datatypes.bool)
+        | string   => eq_dec (A := String.string)
+        | list σ   => eq_dec (A := Datatypes.list (Val σ))
+        | prod σ τ => eq_dec (A := Datatypes.prod (Val σ) (Val τ))
+        | sum σ τ  => eq_dec (A := Datatypes.sum (Val σ) (Val τ))
+        | unit     => eq_dec (A := Datatypes.unit)
+        (* | enum E   => eq_dec (A := enumt E) *)
+        | bvec n   => eq_dec (A := bv n)
+        (* | tuple σs => ctx.Ctx_rect *)
+        (*                 (fun τs => EqDec (EnvRec Val τs)) *)
+        (*                 (eq_dec (A := Datatypes.unit)) *)
+        (*                 (fun τs IHτs τ => *)
+        (*                    @eq_dec *)
+        (*                      (Datatypes.prod (EnvRec Val τs) (Val τ)) *)
+        (*                      (prod_eqdec IHτs (eqd τ))) *)
+        (*                 σs *)
+        (* | union U  => eq_dec (A := uniont U) *)
+        (* | record R => eq_dec (A := recordt R) *)
+        end.
 
-    Lemma unionv_unfold_inj {U} (v1 v2 : Val (union U)) :
-      unionv_unfold U v1 = unionv_unfold U v2 <-> v1 = v2.
-    Proof.
-      split; intro H; [|now f_equal].
-      apply (f_equal (unionv_fold U)) in H.
-      now rewrite !unionv_fold_unfold in H.
-    Qed.
+        #[export] Instance RelVal_eq_dec : forall σ, EqDec (RelVal σ) :=
+      fix eqd σ :=
+        match σ with
+        | int      => eq_dec (A := Z)
+        | bool     => eq_dec (A := Datatypes.bool)
+        | string   => eq_dec (A := String.string)
+        | list σ   => eq_dec (A := Datatypes.list (Val σ))
+        | prod σ τ => eq_dec (A := Datatypes.prod (Val σ) (Val τ))
+        | sum σ τ  => eq_dec (A := Datatypes.sum (Val σ) (Val τ))
+        | unit     => eq_dec (A := Datatypes.unit)
+        (* | enum E   => eq_dec (A := enumt E) *)
+        | bvec n   => eq_dec (A := bv n)
+        (* | tuple σs => ctx.Ctx_rect *)
+        (*                 (fun τs => EqDec (EnvRec Val τs)) *)
+        (*                 (eq_dec (A := Datatypes.unit)) *)
+        (*                 (fun τs IHτs τ => *)
+        (*                    @eq_dec *)
+        (*                      (Datatypes.prod (EnvRec Val τs) (Val τ)) *)
+        (*                      (prod_eqdec IHτs (eqd τ))) *)
+        (*                 σs *)
+        (* | union U  => eq_dec (A := uniont U) *)
+        (* | record R => eq_dec (A := recordt R) *)
+        end.
 
-    Lemma recordv_fold_inj {R} (v1 v2 : NamedEnv Val (recordf_ty R)) :
-      recordv_fold R v1 = recordv_fold R v2 <-> v1 = v2.
-    Proof.
-      split; intro H; [|now f_equal].
-      apply (f_equal (recordv_unfold R)) in H.
-      now rewrite !recordv_unfold_fold in H.
-    Qed.
+    (* Lemma unionv_fold_inj {U} (v1 v2 : {K : unionk U & Val (unionk_ty U K)}) : *)
+    (*   unionv_fold U v1 = unionv_fold U v2 <-> v1 = v2. *)
+    (* Proof. *)
+    (*   split; intro H; [|now f_equal]. *)
+    (*   apply (f_equal (unionv_unfold U)) in H. *)
+    (*   now rewrite !unionv_unfold_fold in H. *)
+    (* Qed. *)
 
-    Lemma recordv_unfold_inj {R} (v1 v2 : Val (ty.record R)) :
-      recordv_unfold R v1 = recordv_unfold R v2 <-> v1 = v2.
-    Proof.
-      split; intro H; [|now f_equal].
-      apply (f_equal (recordv_fold R)) in H.
-      now rewrite ?recordv_fold_unfold in H.
-    Qed.
+    (* Lemma unionv_unfold_inj {U} (v1 v2 : Val (union U)) : *)
+    (*   unionv_unfold U v1 = unionv_unfold U v2 <-> v1 = v2. *)
+    (* Proof. *)
+    (*   split; intro H; [|now f_equal]. *)
+    (*   apply (f_equal (unionv_fold U)) in H. *)
+    (*   now rewrite !unionv_fold_unfold in H. *)
+    (* Qed. *)
+
+    (* Lemma recordv_fold_inj {R} (v1 v2 : NamedEnv Val (recordf_ty R)) : *)
+    (*   recordv_fold R v1 = recordv_fold R v2 <-> v1 = v2. *)
+    (* Proof. *)
+    (*   split; intro H; [|now f_equal]. *)
+    (*   apply (f_equal (recordv_unfold R)) in H. *)
+    (*   now rewrite !recordv_unfold_fold in H. *)
+    (* Qed. *)
+
+    (* Lemma recordv_unfold_inj {R} (v1 v2 : Val (ty.record R)) : *)
+    (*   recordv_unfold R v1 = recordv_unfold R v2 <-> v1 = v2. *)
+    (* Proof. *)
+    (*   split; intro H; [|now f_equal]. *)
+    (*   apply (f_equal (recordv_fold R)) in H. *)
+    (*   now rewrite ?recordv_fold_unfold in H. *)
+    (* Qed. *)
 
     Lemma K (σ : Ty) (p : σ = σ) : p = eq_refl.
     Proof. apply uip. Qed.
